proof/rejection_sampling/UniformSampling_Concrete_LF.ec
@@ -12,7 +12,7 @@ module M1 = W64_SchnorrExtract_ct.M(W64_SchnorrExtract_ct.Syscall).
 
 
 lemma rsample_leakages2 a  &m : (glob M1){m} = [] =>
-  Pr[ M1.rsample(a) @ &m : M1.leakages <> samp_t res.`1 ] = 0%r.
+  Pr[ M1.bn_rsample(a) @ &m : M1.leakages <> samp_t res.`1 ] = 0%r.
 progress. byphoare (_: glob M1 = [] ==> _).
 hoare. simplify.
 conseq (rsample_leakages []). auto. smt(@List).  auto. auto.
@@ -20,35 +20,35 @@ qed.
 
 (* samp_t_correct *)
 lemma samp_t_correct a l x &m : (glob M1){m} = [] =>
-  Pr[ M1.rsample(a) @ &m : M1.leakages = l  /\ res.`2 = x ]
-  = Pr[ M1.rsample(a) @ &m : l = samp_t res.`1 /\ res.`2 = x  ].
+  Pr[ M1.bn_rsample(a) @ &m : M1.leakages = l  /\ res.`2 = x ]
+  = Pr[ M1.bn_rsample(a) @ &m : l = samp_t res.`1 /\ res.`2 = x  ].
 move => H.
-have ->: Pr[ M1.rsample(a) @ &m : l = samp_t res.`1 /\ res.`2 = x ]
- = Pr[ M1.rsample(a) @ &m : l = samp_t res.`1 /\ res.`2 = x /\ M1.leakages = samp_t res.`1  ].
-  have -> : Pr[M1.rsample(a) @ &m : l = samp_t res.`1 /\ res.`2 = x]
-   = Pr[M1.rsample(a) @ &m : l = samp_t res.`1 /\ res.`2 = x /\ M1.leakages = samp_t res.`1]
-   + Pr[M1.rsample(a) @ &m : l = samp_t res.`1 /\ res.`2 = x /\ M1.leakages <> samp_t res.`1].
+have ->: Pr[ M1.bn_rsample(a) @ &m : l = samp_t res.`1 /\ res.`2 = x ]
+ = Pr[ M1.bn_rsample(a) @ &m : l = samp_t res.`1 /\ res.`2 = x /\ M1.leakages = samp_t res.`1  ].
+  have -> : Pr[M1.bn_rsample(a) @ &m : l = samp_t res.`1 /\ res.`2 = x]
+   = Pr[M1.bn_rsample(a) @ &m : l = samp_t res.`1 /\ res.`2 = x /\ M1.leakages = samp_t res.`1]
+   + Pr[M1.bn_rsample(a) @ &m : l = samp_t res.`1 /\ res.`2 = x /\ M1.leakages <> samp_t res.`1].
    rewrite Pr[mu_split (M1.leakages = samp_t res.`1)]. smt(). 
-  have ->: Pr[M1.rsample(a) @ &m :
+  have ->: Pr[M1.bn_rsample(a) @ &m :
    l = samp_t res.`1 /\ res.`2 = x /\ M1.leakages <> samp_t res.`1] = 0%r.
-    have : Pr[M1.rsample(a) @ &m :
+    have : Pr[M1.bn_rsample(a) @ &m :
        l = samp_t res.`1 /\ res.`2 = x /\ M1.leakages <> samp_t res.`1]
-     <= Pr[ M1.rsample(a) @ &m : M1.leakages <> samp_t res.`1 ]. smt(@Distr).
+     <= Pr[ M1.bn_rsample(a) @ &m : M1.leakages <> samp_t res.`1 ]. smt(@Distr).
     rewrite (rsample_leakages2 a &m). auto. smt(@Distr). 
 auto.
-have -> : Pr[ M1.rsample(a) @ &m : l = samp_t res.`1 /\ res.`2 = x /\ M1.leakages = samp_t res.`1  ]
- = Pr[ M1.rsample(a) @ &m : res.`2 = x /\  l = M1.leakages /\ M1.leakages = samp_t res.`1  ].
+have -> : Pr[ M1.bn_rsample(a) @ &m : l = samp_t res.`1 /\ res.`2 = x /\ M1.leakages = samp_t res.`1  ]
+ = Pr[ M1.bn_rsample(a) @ &m : res.`2 = x /\  l = M1.leakages /\ M1.leakages = samp_t res.`1  ].
 rewrite Pr[mu_eq]. move => &hr. split.  smt().  smt(). auto.
-have -> : Pr[ M1.rsample(a) @ &m : res.`2 = x /\ l = M1.leakages /\ M1.leakages = samp_t res.`1  ]
- = Pr[ M1.rsample(a) @ &m :  l = M1.leakages /\ res.`2 = x ].
-  have : Pr[ M1.rsample(a) @ &m :  l = M1.leakages /\ res.`2 = x ] 
-   = Pr[ M1.rsample(a) @ &m :  l = M1.leakages /\ res.`2 = x /\ M1.leakages = samp_t res.`1  ]
-   + Pr[ M1.rsample(a) @ &m :  l = M1.leakages /\ res.`2 = x /\ M1.leakages <> samp_t res.`1  ].
+have -> : Pr[ M1.bn_rsample(a) @ &m : res.`2 = x /\ l = M1.leakages /\ M1.leakages = samp_t res.`1  ]
+ = Pr[ M1.bn_rsample(a) @ &m :  l = M1.leakages /\ res.`2 = x ].
+  have : Pr[ M1.bn_rsample(a) @ &m :  l = M1.leakages /\ res.`2 = x ] 
+   = Pr[ M1.bn_rsample(a) @ &m :  l = M1.leakages /\ res.`2 = x /\ M1.leakages = samp_t res.`1  ]
+   + Pr[ M1.bn_rsample(a) @ &m :  l = M1.leakages /\ res.`2 = x /\ M1.leakages <> samp_t res.`1  ].
  rewrite Pr[mu_split (M1.leakages = samp_t res.`1 )]. smt().
-   have : Pr[ M1.rsample(a) @ &m :  l = M1.leakages /\ res.`2 = x /\ M1.leakages <> samp_t res.`1  ]
+   have : Pr[ M1.bn_rsample(a) @ &m :  l = M1.leakages /\ res.`2 = x /\ M1.leakages <> samp_t res.`1  ]
     = 0%r.
-     have : Pr[ M1.rsample(a) @ &m :  l = M1.leakages /\ res.`2 = x /\ M1.leakages <> samp_t res.`1  ] 
-         <= Pr[ M1.rsample(a) @ &m : M1.leakages <> samp_t res.`1 ].
+     have : Pr[ M1.bn_rsample(a) @ &m :  l = M1.leakages /\ res.`2 = x /\ M1.leakages <> samp_t res.`1  ] 
+         <= Pr[ M1.bn_rsample(a) @ &m : M1.leakages <> samp_t res.`1 ].
        rewrite Pr[mu_sub]. auto. auto.
     rewrite (rsample_leakages2 a &m). auto. smt(@Distr).
     move => h. rewrite h. simplify. progress. rewrite H0.
@@ -58,15 +58,15 @@ qed.
 
 
 (* rsample_leakf *)
-lemma rsample_leakf a x l &m : (glob M1){m} = [] 
- => Pr[ M1.rsample(a) @ &m : M1.leakages = l /\ res.`2 = x  ]
-  = Pr[ M1.rsample(a) @ &m :  (inv (-1) samp_t) l = res.`1  /\ res.`2 = x  ].
+lemma bn_rsample_leakf a x l &m : (glob M1){m} = [] 
+ => Pr[ M1.bn_rsample(a) @ &m : M1.leakages = l /\ res.`2 = x  ]
+  = Pr[ M1.bn_rsample(a) @ &m :  (inv (-1) samp_t) l = res.`1  /\ res.`2 = x  ].
 move => ic (* ic' *). rewrite  (samp_t_correct a l x &m). auto. auto.
 simplify. 
 have -> : 
-  Pr[M1.rsample(a) @ &m :
+  Pr[M1.bn_rsample(a) @ &m :
    l = samp_t res.`1 /\ res.`2 = x]
-  =   Pr[M1.rsample(a) @ &m :
+  =   Pr[M1.bn_rsample(a) @ &m :
    l = samp_t res.`1 /\ res.`2 = x /\ 0 <= res.`1]. byequiv.
 proc. wp. simplify. 
 while (0 <= i{1} /\ ={i,byte_p, byte_z}). wp.  simplify.
@@ -76,9 +76,9 @@ call (_:true). wp. sim. wp.
 skip. progress. smt(). wp. 
 call (_:true). wp. sim. wp.  skip. progress.
 auto. auto.
-have -> : Pr[M1.rsample(a) @ &m :
+have -> : Pr[M1.bn_rsample(a) @ &m :
    inv (-1) samp_t l = res.`1 /\ res.`2 = x] 
- = Pr[M1.rsample(a) @ &m :
+ = Pr[M1.bn_rsample(a) @ &m :
    inv (-1) samp_t l = res.`1 /\ res.`2 = x /\ 0 <= res.`1].
  byequiv.
 proc. wp. simplify.
@@ -106,7 +106,7 @@ require import W64_SchnorrExtract.
 module M2 = W64_SchnorrExtract.M(W64_SchnorrExtract.Syscall).  
 
 lemma M1_M2_rsample :
-  equiv  [ M1.rsample ~ M2.rsample 
+  equiv  [ M1.bn_rsample ~ M2.bn_rsample 
     : ={arg} ==> ={res}  ].
 proof. proc.  sim. 
 call (_:true). 
@@ -122,10 +122,10 @@ require import UniformSampling_Concrete.
 
 
 equiv rsample_cspec_equiv:
- M1.rsample ~ CSpecFp.rsample:
+ M1.bn_rsample ~ CSpecFp.rsample:
   W64xN.valR byte_z{1} = a{2}
   ==> W64xN.valR res{1}.`2 = res{2}.`2 /\ res{1}.`1 = res{2}.`1.
-transitivity M2.rsample 
+transitivity M2.bn_rsample 
  (={arg} ==> ={res})
  (W64xN.valR byte_z{1} = a{2}
   ==> W64xN.valR res{1}.`2 = res{2}.`2 /\ res{1}.`1 = res{2}.`1).
@@ -136,22 +136,22 @@ qed.
 
 
 lemma rsample_cspec_pr a i x &m : 
-  Pr[ M1.rsample(a) @ &m : res = (i,x)  ]
+  Pr[ M1.bn_rsample(a) @ &m : res = (i,x)  ]
    = Pr[ CSpecFp.rsample(W64xN.valR a) @ &m : res = (i, W64xN.valR x)  ].
 byequiv.
 conseq rsample_cspec_equiv. progress. progress. smt().
 smt(@W64xN). auto. auto.
 qed.
 
-lemma jrsample_pr a i x &m : 
+lemma bn_rsample_pr a i x &m : 
   1 <= i => RSP (W64xN.valR a) (W64xN.valR x) =>
-  Pr[ M1.rsample(a) @ &m : res = (i,x) ]
+  Pr[ M1.bn_rsample(a) @ &m : res = (i,x) ]
    = mu D (predC (RSP (W64xN.valR a))) ^ (i - 1) * mu1 D (W64xN.valR x).
 rewrite rsample_cspec_pr.
 apply rsample_pr. 
 qed.
 
-lemma rsample_index_pos &m a : Pr[M1.rsample(a) @ &m : res.`1 <= 0 ] = 0%r.
+lemma rsample_index_pos &m a : Pr[M1.bn_rsample(a) @ &m : res.`1 <= 0 ] = 0%r.
 byphoare (_: arg = a ==> _);auto. hoare.
 proc.  simplify.
 unroll 18. rcondt 18. wp. wp. 
@@ -174,22 +174,22 @@ op g a l : real
 
 
         
-lemma jrsample_v &m x a l: (glob M1){m} = [] 
-  => Pr[ M1.rsample(a) @ &m : M1.leakages = l  /\ res.`2 = x  ] 
+lemma bn_rsample_v &m x a l: (glob M1){m} = [] 
+  => Pr[ M1.bn_rsample(a) @ &m : M1.leakages = l  /\ res.`2 = x  ] 
        = if (valR a <= valR x) then 0%r else (g a l).
       progress.
-   rewrite  (rsample_leakf a x l &m);auto.
+   rewrite  (bn_rsample_leakf a x l &m);auto.
 case (inv (-1) samp_t l <= 0). 
 move => q. rewrite /g. rewrite q.  simplify. 
-  have : Pr[M1.rsample(a) @ &m :
+  have : Pr[M1.bn_rsample(a) @ &m :
    inv (-1) samp_t l = res.`1 /\ res.`2 = x] 
-    <= Pr[M1.rsample(a) @ &m : res.`1 <= 0 ]. simplify. rewrite Pr[mu_sub]. smt().
+    <= Pr[M1.bn_rsample(a) @ &m : res.`1 <= 0 ]. simplify. rewrite Pr[mu_sub]. smt().
    auto. smt(rsample_index_pos @Distr).
 move => q.
 have -> : 
- Pr[M1.rsample(a) @ &m :
+ Pr[M1.bn_rsample(a) @ &m :
    inv (-1) samp_t l = res.`1 /\ res.`2 = x]
-  = Pr[M1.rsample(a) @ &m :
+  = Pr[M1.bn_rsample(a) @ &m :
    res = (inv (-1) samp_t l , x) ]. rewrite Pr[mu_eq]. smt(). auto.
 case (valR x < valR a) => case1.
 rewrite rsample_cspec_pr.
@@ -200,9 +200,9 @@ have ->: mu1 D (W64xN.valR x) = 1%r / Ring_ops_spec.M%r.
 rewrite duniform1E_uniq. smt(@List).
  have f1 : 0 <= W64xN.valR x < Ring_ops_spec.M. smt(@W64xN).  smt(@Distr @List). 
 rewrite /g.   smt().
-have : Pr[W64_SchnorrExtract_ct.M(W64_SchnorrExtract_ct.Syscall).rsample(a) @ &m :
+have : Pr[W64_SchnorrExtract_ct.M(W64_SchnorrExtract_ct.Syscall).bn_rsample(a) @ &m :
    res.`2 = x] = 0%r.
-  have -> : Pr[W64_SchnorrExtract_ct.M(W64_SchnorrExtract_ct.Syscall).rsample(a) @ &m :
+  have -> : Pr[W64_SchnorrExtract_ct.M(W64_SchnorrExtract_ct.Syscall).bn_rsample(a) @ &m :
      res.`2 =  x] = Pr[ CSpecFp.rsample(W64xN.valR a) @ &m : res.`2 =  W64xN.valR x ].
   byequiv. conseq rsample_cspec_equiv. auto. progress. rewrite H0.  auto.  smt(@W64xN). auto. auto.
   apply rsample_pr_out. auto.
@@ -211,11 +211,11 @@ qed.
 
 op h a : real = 1%r/(valR a)%r. 
 
-lemma jrsample_w &m x a: 
- Pr[ M1.rsample(a) @ &m : res.`2 = x ] 
+lemma bn_rsample_w &m x a: 
+ Pr[ M1.bn_rsample(a) @ &m : res.`2 = x ] 
   = if (valR a <= valR x) then 0%r else h a.    
 proof. 
- have ->: Pr[ M1.rsample(a) @ &m : res.`2 = x ] =
+ have ->: Pr[ M1.bn_rsample(a) @ &m : res.`2 = x ] =
   Pr[ CSpecFp.rsample(W64xN.valR a) @ &m : res.`2 =  W64xN.valR x ].
   byequiv. conseq rsample_cspec_equiv. auto. 
 progress. rewrite - H. auto. smt(@W64xN). auto. auto.
@@ -229,9 +229,9 @@ qed.
 
 op rsample_f a l = h a / g a l.
 
-lemma jrsample_leakfree pin l a &m: (glob M1){m} = [] 
- =>  let v = Pr[ M1.rsample(pin) @ &m : res.`2 = a  ] in 
-     let w = Pr[ M1.rsample(pin) @ &m : M1.leakages = l  /\ res.`2 = a  ] in 
+lemma bn_rsample_leakfree pin l a &m: (glob M1){m} = [] 
+ =>  let v = Pr[ M1.bn_rsample(pin) @ &m : res.`2 = a  ] in 
+     let w = Pr[ M1.bn_rsample(pin) @ &m : M1.leakages = l  /\ res.`2 = a  ] in 
   0%r < w => v/w 
   = rsample_f pin l.
 move => l_empty v w f1.
@@ -239,14 +239,14 @@ have : (valR a < valR pin).
  case (valR pin <= valR a) => h.
  have : w <= 0%r.
  rewrite /w.  
- rewrite (jrsample_v &m a pin l _). auto.
+ rewrite (bn_rsample_v &m a pin l _). auto.
  rewrite h. auto.
  smt(). 
  smt().
 move => a_less_pin.
 rewrite /f.
-rewrite  (jrsample_v &m a pin l _). auto.
-rewrite  (jrsample_w &m a pin ). auto. 
+rewrite  (bn_rsample_v &m a pin l _). auto.
+rewrite  (bn_rsample_w &m a pin ). auto. 
 smt().
 qed.
 
